Remove isLambda condition on fixpoint bodies

template-coq/theories/Typing.v
@@ -80,13 +80,7 @@ Definition fix_subst (l : mfixpoint term) :=
 
 Definition unfold_fix (mfix : mfixpoint term) (idx : nat) :=
   match List.nth_error mfix idx with
-  | Some d =>
-    if isLambda d.(dbody) then
-      Some (d.(rarg), subst0 (fix_subst mfix) d.(dbody))
-    else None (* We don't unfold ill-formed fixpoints, which would
-                 render confluence unprovable, creating an infinite
-                 number of critical pairs between unfoldings of fixpoints.
-                 e.g. [fix f := f] is not allowed. *)
+  | Some d => Some (d.(rarg), subst0 (fix_subst mfix) d.(dbody))
   | None => None
   end.
 
@@ -951,8 +945,7 @@ Inductive typing `{checker_flags} (Σ : global_env_ext) (Γ : context) : term ->
     nth_error mfix n = Some decl ->
     wf_local Σ Γ ->
     All (fun d => {s & Σ ;;; Γ |- d.(dtype) :  tSort s}) mfix ->
-    All (fun d => (Σ ;;; Γ ,,, fix_context mfix |- d.(dbody) : lift0 #|fix_context mfix| d.(dtype))
-      * (isLambda d.(dbody) = true)%type) mfix ->
+    All (fun d => (Σ ;;; Γ ,,, fix_context mfix |- d.(dbody) : lift0 #|fix_context mfix| d.(dtype))) mfix ->
     wf_fixpoint Σ mfix ->
       Σ ;;; Γ |- tFix mfix n : decl.(dtype)
 
@@ -1067,7 +1060,7 @@ Proof.
   - exact (S (S (wf_local_size _ typing_size _ a))).
   - exact (S (Nat.max d1 (Nat.max d2
       (all2_size _ (fun x y p => Nat.max (typing_size Σ Γ (snd x) (snd y) (snd (fst p))) (typing_size _ _ _ _ (snd p))) a)))).
-  - exact (S (Nat.max (Nat.max (wf_local_size _ typing_size _ a) (all_size _ (fun x  p => typing_size Σ _ _ _ p.π2) a0)) (all_size _ (fun x p => typing_size Σ _ _ _ (fst p)) a1))).
+  - exact (S (Nat.max (Nat.max (wf_local_size _ typing_size _ a) (all_size _ (fun x  p => typing_size Σ _ _ _ p.π2) a0)) (all_size _ (fun x p => typing_size Σ _ _ _ p) a1))).
   - exact (S (Nat.max (Nat.max (wf_local_size _ typing_size _ a) (all_size _ (fun x  p => typing_size Σ _ _ _ p.π2) a0)) (all_size _ (fun x p => typing_size Σ _ _ _ p) a1))).
 Defined.
 
@@ -1299,7 +1292,6 @@ Lemma typing_ind_env `{cf : checker_flags} :
         All_local_env_over typing Pdecl Σ Γ wfΓ ->
         All (fun d => {s & (Σ ;;; Γ |- d.(dtype) : tSort s)%type * P Σ Γ d.(dtype) (tSort s)})%type mfix ->
         All (fun d => (Σ ;;; Γ ,,, types |- d.(dbody) : lift0 #|types| d.(dtype))%type *
-                   (isLambda d.(dbody) = true)%type *
             P Σ (Γ ,,, types) d.(dbody) (lift0 #|types| d.(dtype)))%type mfix ->
         wf_fixpoint Σ.1 mfix ->
         P Σ Γ (tFix mfix n) decl.(dtype)) ->
@@ -1562,8 +1554,8 @@ Proof.
                 typing_size Hty <
                       S
                         (all_size (fun x : def term => (Σ;;; Γ ,,, fix_context mfix |- dbody x : lift0 #|fix_context mfix| (dtype x))%type
-                                                        * (isLambda (dbody x) = true)%type)%type
-                                   (fun (x : def term) p => typing_size (fst p)) a1) ->
+                                                       )%type
+                                   (fun (x : def term) p => typing_size p) a1) ->
                        Forall_decls_typing P Σ.1 * P Σ Γ0 t T).
         {intros. eapply (X14 _ X _ _ Hty); eauto. lia. }
         clear X14 X13.
@@ -1572,7 +1564,7 @@ Proof.
 
         induction a1; econstructor; eauto.
         ++ split; auto.
-          eapply (X _ (typing_wf_local (fst p)) _ _ (fst p)). simpl. lia.
+          eapply (X _ (typing_wf_local p) _ _ p). simpl. lia.
         ++ eapply IHa1. intros.
           eapply (X _ X0 _ _ Hty). simpl; lia.
 
